src/custard/FStarC.Custard.Syntax.fsti
@@ -174,7 +174,7 @@ type flag =
 type tydef =
   | TAbbrev  of cty
   | TRecord  of list (string & cty)
-  | TVariant of list (string & list (string & cty))
+  | TVariant of list (name & list (string & cty))
   | TAbstract
 
 type dtype = {
