tests/custard/Recursion.fst
@@ -1,0 +1,10 @@
+module Recursion
+open FStar.All
+open FStar.IO
+
+let rec fact (n:nat) : nat =
+  if n = 0 then 1 else n * fact (n - 1)
+
+let main () : ML unit =
+  print_string (string_of_int (fact 5));
+  print_string "\n"
